theories/elpi_valid_state.v
@@ -8,6 +8,17 @@ From det Require Import zify_ssreflect.
 Section NurValidState.
   Variable u : Unif.
 
+
+  (* Give a list, 
+     I have two cuts in 2 different disjuncts: [.... !1 .....] Y0 ... Yn [.... !2 ....] X0 X1 ... Xn
+     The second cut points to a suffix Xn, it means that
+     - the first cut cannot point to X0 X1 ... X(n-1), beacause:
+       - either it is a cut generated at the same level of the second cut
+         and therefore the two cuts point EXACTLY to the same stuff
+       - or it is a cut generated more deeply then the second cut,
+         therefore it should point to something between `Y0 ... Yn [.... !2 ....]`
+     - to sum up, the first cut point to the intervale [Y0 ... Yn] + [... !2 ...] + Xn
+  *)
   Fixpoint valid_caG (gs:goals) (a:alts) (bt:alts) {struct gs} :=
     match gs with
     | no_goals => true
